Update coherence for mutual recursion.

Coherence/Coherence.v
@@ -2,118 +2,67 @@ Require Import CSet Le.
 
 Require Import Plus Util AllInRel Map.
 Require Import Val Var Env EnvTy IL Annotation Liveness Restrict Bisim MoreExp SetOperations.
-Require Import DecSolve RenamedApart LabelsDefined.
+Require Import DecSolve RenamedApart LabelsDefined InRel.
 
 Set Implicit Arguments.
 
 (** * Definition of Coherence: [srd] *)
 
+Definition global (F:params*stmt) (alF:ann (set var)) := getAnn alF \ of_list (fst F).
+Definition globals (F:list (params*stmt)) (alF:list (ann (set var))) :=
+  zip global F alF.
+Definition oglobals F alF := List.map Some (globals F alF).
+
 Inductive srd : list (option (set var)) -> stmt -> ann (set var) -> Prop :=
- | srdExp DL x e s lv al
-    : srd (restrict DL (lv\{{x}})) s al
+| srdExp DL x e s lv al
+  : srd (restrict DL (lv\{{x}})) s al
     -> srd DL (stmtLet x e s) (ann1 lv al)
-  | srdIf DL e s t lv als alt
-    : srd DL s als
+| srdIf DL e s t lv als alt
+  : srd DL s als
     -> srd DL t alt
     -> srd DL (stmtIf e s t) (ann2 lv als alt)
-  | srdRet e DL lv
-    : srd DL (stmtReturn e) (ann0 lv)
-  | srdGoto DL lv G' f Y
-    : get DL (counted f) (Some G')
+| srdRet e DL lv
+  : srd DL (stmtReturn e) (ann0 lv)
+| srdGoto DL lv G' f Y
+  : get DL (counted f) (Some G')
     -> srd DL (stmtApp f Y) (ann0 lv)
- | srdExtern DL x f Y s lv al
-    : srd (restrict DL (lv\{{x}})) s al
+| srdExtern DL x f Y s lv al
+  : srd (restrict DL (lv\{{x}})) s al
     -> srd DL (stmtExtern x f Y s) (ann1 lv al)
-  | srdLet DL s t Z lv als alt
-    : srd (restrict (Some (getAnn als \ of_list Z)::DL) (getAnn als \ of_list Z))
-          s als
-    -> srd (Some (getAnn als \ of_list Z)::DL) t alt
-    -> srd DL (stmtFun Z s t) (ann2 lv als alt).
-
-(*
-Definition peq := prod_eq (@feq var var eq) (@Equal var _ _).
-
-Instance srd_morphism
-  : Proper (list_eq (option_eq Equal) ==> Equal ==> eq ==> impl) srd.
-Proof.
-  unfold Proper, peq, respectful, impl; intros; decompose records; simpl in *; subst.
-  general induction H2; simpl in *; eauto using srd.
-  + econstructor; eauto.
-    - rewrite <- H1; eauto.
-    - eapply IHsrd. rewrite H0. rewrite <- H1. reflexivity.
-      rewrite H1. reflexivity.
-
-  + econstructor; eauto. rewrite <- H1; eauto.
-  + econstructor; eauto. rewrite <- H1; eauto.
-
-  + edestruct (list_eq_get H2 H0); decompose records;
-    destruct x; simpl in * |- *; eauto; inv H6.
-    econstructor; eauto. rewrite <- H3; eauto.
-    rewrite <- H3, <- H8; eauto.
-
-  + econstructor; eauto. rewrite <- H1; eauto.
-    eapply IHsrd1; eauto; try reflexivity.
-    econstructor; eauto. reflexivity.
-    rewrite H0. reflexivity.
-    eapply IHsrd2; eauto. constructor; eauto; reflexivity.
-Qed.
-*)
+| srdLet DL F t lv als alt
+  : length F = length als
+    -> (forall n Zs a, get F n Zs -> get als n a ->
+                 srd (restrict (oglobals F als ++ DL)
+                               (getAnn a \ of_list (fst Zs))) (snd Zs) a)
+    -> srd (oglobals F als ++ DL) t alt
+    -> srd DL (stmtFun F t) (annF lv als alt).
 
 (** ** Coherence is decidable *)
 
 Definition srd_dec DL s a
   : Computable (srd DL s a).
 Proof.
-  hnf.
-  general induction s; simpl.
-  + edestruct a as [|lv a'|]; try dec_solve.
-    edestruct (IHs (restrict DL (lv\{{x}})) a'); try dec_solve.
-  + edestruct a as [?|?|lv als alt]; try dec_solve.
-    edestruct (IHs1 DL als), (IHs2 DL alt); try dec_solve.
+  hnf. revert DL a.
+  sinduction s; simpl.
+  + edestruct a as [|lv a'| |]; try dec_solve.
+    edestruct (X x0); try dec_solve; eauto.
+  + edestruct a as [?|?|lv als alt|]; try dec_solve.
+    edestruct (X x1), (X x2); try dec_solve; eauto.
   + destruct a;
     destruct (get_dec DL (counted l)) as [[[G'|] ?]|?];
     try dec_solve.
   + destruct a; try dec_solve.
-  + edestruct a as [|lv a'|]; try dec_solve.
-    edestruct (IHs (restrict DL (lv\{{x}})) a'); try dec_solve.
-  + destruct a as [?|?|lv als alt]; try dec_solve.
-    edestruct (IHs1 (restrict (Some (getAnn als \ of_list Z)::DL) (getAnn als \ of_list Z)) als);
-    edestruct (IHs2 (Some (getAnn als \ of_list Z)::DL) alt); try dec_solve.
+  + edestruct a as [|lv a'| |]; try dec_solve.
+    edestruct (X x0); try dec_solve; eauto.
+  + destruct a as [?|?|lv als alt| ]; try dec_solve.
+    decide (length s = length sa); try dec_solve.
+    edestruct (X x) with (DL:=oglobals s sa++DL); eauto; try dec_solve.
+    edestruct (indexwise_R_dec'
+                 (R:=fun x y => srd (restrict (oglobals s sa ++ DL) (getAnn y \ of_list (fst x))) (snd x) y) (LA:=s) (LB:=sa));
+      try dec_solve.
+    intros. eapply X; eauto.
+    Grab Existential Variables. eauto. eauto. eauto. eauto.
 Defined.
-
-(*
-Fixpoint freeVar_live (s:stmt) : ann (set var) :=
-  match s with
-    | stmtLet x e s0 => ann1 (freeVars s) (freeVar_live s0)
-    | stmtIf x s1 s2 => ann2 (freeVars s) (freeVar_live s1) (freeVar_live s2)
-    | stmtApp l Y => ann0 (freeVars s)
-    | stmtReturn x => ann0 (freeVars s)
-    | stmtFun Z s1 s2 => ann2 (freeVars s) (freeVar_live s1) (freeVar_live s2)
-  end.
-
-Lemma  getAnn_freeVar_live (s:stmt)
-  : getAnn (freeVar_live s) = freeVars s.
-Proof.
-  destruct s; eauto.
-Qed.
-
-
-Lemma free_live_sound s Lv DL D G
-  : (forall n blv Z, get Lv n (blv, Z) -> of_list Z ⊆ blv)
-  -> srd DL (D, G) s
-  -> live_sound Lv s (freeVar_live s).
-Proof.
-  intros. general induction H0; simpl in * |- *.
-  econstructor. eapply IHsrd; eauto. eapply union_subset_2.
-  rewrite getAnn_freeVar_live. eapply union_subset_1.
-  econstructor; eauto. eapply union_subset_2; cset_tac; eauto.
-  rewrite getAnn_freeVar_live. eapply Subset_trans; eauto; eapply union_subset_1.
-  rewrite getAnn_freeVar_live. eapply Subset_trans; eauto. eapply union_subset_1.
-  rewrite union_comm. eapply union_subset_1.
-  econstructor. cset_tac; eauto.
-  econstructor. (* here is the counterexample *)
-Abort.
-*)
 
 (** ** Some monotonicity properties *)
 
@@ -123,17 +72,18 @@ Lemma srd_monotone (DL DL' : list (option (set var))) s a
    -> srd DL' s a.
 Proof.
   intros. general induction H; eauto using srd.
-  + econstructor.
+  - econstructor.
     eapply IHsrd; eauto. eapply restrict_subset; eauto.
-  + destruct (PIR2_nth H0 H); eauto; dcr. inv H3.
+  - destruct (PIR2_nth H0 H); eauto; dcr. inv H3.
     econstructor; eauto.
-  + econstructor. eapply IHsrd; eauto.
+  - econstructor. eapply IHsrd; eauto.
     eapply restrict_subset; eauto.
-  + econstructor; eauto.
-    eapply IHsrd1. repeat rewrite restrict_incl; try reflexivity.
-    constructor; eauto. reflexivity.
-    eapply restrict_subset; eauto.
-    eapply IHsrd2. constructor; eauto. reflexivity.
+  - econstructor; eauto.
+    + intros. eapply H1; eauto.
+      repeat rewrite restrict_app.
+      eapply PIR2_app; eauto.
+      eapply restrict_subset; eauto.
+    + eapply IHsrd. eapply PIR2_app; eauto.
 Qed.
 
 Lemma srd_monotone2 (DL DL' : list (option (set var))) s a
@@ -142,21 +92,61 @@ Lemma srd_monotone2 (DL DL' : list (option (set var))) s a
    -> srd DL' s a.
 Proof.
   intros. general induction H; eauto using srd.
-  + econstructor.
+  - econstructor.
     eapply IHsrd; eauto. eapply restrict_subset2; eauto.
-  + destruct (PIR2_nth H0 H); eauto; dcr. inv H3.
+  - destruct (PIR2_nth H0 H); eauto; dcr. inv H3.
     econstructor; eauto.
-  + econstructor. eapply IHsrd, restrict_subset2; eauto.
-  + econstructor; eauto.
-    eapply IHsrd1. repeat rewrite restrict_incl; try reflexivity.
-    constructor; eauto. reflexivity.
-    eapply restrict_subset2; eauto.
-    eapply IHsrd2. constructor; eauto. reflexivity.
+  - econstructor. eapply IHsrd, restrict_subset2; eauto.
+  - econstructor; eauto.
+    + intros. eapply H1; eauto.
+      repeat rewrite restrict_app.
+      eapply PIR2_app; eauto.
+      eapply restrict_subset2; eauto.
+    + eapply IHsrd. eapply PIR2_app; eauto.
 Qed.
 
 (** *** Every renamed apart program is coherent *)
 (** Note that this lemma also builds the liveness annotation:
     It exploits that we can always claim more variables live *)
+
+Hint Extern 20 =>
+match goal with
+  | [ H: length ?L = length ?L' |- length ?L = length (List.map ?f ?L')] => rewrite map_length; eauto
+end.
+
+Lemma get_bounded L D
+: (forall n x, get L n (Some x) -> x ⊆ D)
+  -> bounded L D.
+Proof.
+  general induction L; simpl; isabsurd; eauto.
+  destruct a; eauto 50 using get.
+Qed.
+
+Lemma inv_oglobals F als k lv
+: length F = length als
+  -> get (oglobals F als) k ⎣lv⎦
+  -> exists Zs a, get F k Zs /\ get als k a /\ lv = getAnn a \ of_list (fst Zs).
+Proof.
+  intros. length_equify.
+  general induction H; isabsurd.
+  - inv H0.
+    + eexists; eauto using get.
+    + edestruct IHlength_eq as [? []]; eauto; dcr; subst.
+      do 2 eexists; eauto using get.
+Qed.
+
+Lemma inv_globals F als k lv
+: length F = length als
+  -> get (globals F als) k lv
+  -> exists Zs a, get F k Zs /\ get als k a /\ lv = getAnn a \ of_list (fst Zs).
+Proof.
+  intros. length_equify.
+  general induction H; isabsurd.
+  - inv H0.
+    + eexists; eauto using get.
+    + edestruct IHlength_eq as [? []]; eauto; dcr; subst.
+      do 2 eexists; eauto using get.
+Qed.
 
 Lemma renamedApart_coherent s ang DL
 : renamedApart s ang
@@ -185,29 +175,80 @@ Proof.
     rewrite H2. simpl in *. rewrite <- incl_add'; eauto.
     erewrite bounded_restrict_eq; simpl; eauto.
     simpl. cset_tac; intuition.
-  - econstructor.
-    + eapply srd_monotone.
-      eapply (IHrenamedApart1 (D::DL)); eauto using labelsDefined.
-      rewrite H3. simpl in *. rewrite <- incl_right.
-      split; eauto; reflexivity.
+  - econstructor; eauto.
+    + intros. inv_map H10.
+      exploit H1; eauto. instantiate (1:=globals F (List.map (mapAnn fst) ans) ++ DL).
+      rewrite app_length. unfold globals. rewrite zip_length2; eauto.
+      exploit H2; eauto; dcr.
+      rewrite List.map_app. eapply bounded_app; split; eauto.
+      rewrite H15. eapply get_bounded.
+      intros. inv_map H18. eapply inv_globals in H20.
+      destruct H20; dcr; subst.
+      inv_map H21. exploit H2; eauto; dcr.
+      rewrite getAnn_mapAnn. rewrite H24.
+      revert H25; clear_all; cset_tac; intuition. rewrite map_length; eauto.
+      rewrite H15. rewrite <- incl_right; eauto.
+      eapply srd_monotone. eapply X.
       rewrite getAnn_mapAnn; simpl.
-      destruct if.
-      * econstructor. econstructor. rewrite H3; simpl.
-        cset_tac; intuition; eauto.
-        simpl in *. rewrite H3; simpl.
-        erewrite bounded_restrict_eq; simpl; eauto.
-        simpl. cset_tac; intuition; eauto.
-      * exfalso. eapply n. rewrite H3; simpl. reflexivity.
-    + eapply srd_monotone.
-      eapply (IHrenamedApart2 (D::DL)); eauto using labelsDefined.
-      rewrite H5. simpl; intuition.
-      rewrite getAnn_mapAnn; simpl.
-      econstructor. econstructor. rewrite H3; simpl.
-      cset_tac; intuition; eauto.
+      repeat rewrite restrict_app. rewrite List.map_app.
+      eapply PIR2_app.
+      erewrite bounded_restrict_eq. reflexivity.
       reflexivity.
+      eapply get_bounded.
+      intros. eapply inv_oglobals in H15.
+      destruct H15; dcr; subst.
+      inv_map H16. exploit H2; eauto; dcr.
+      rewrite getAnn_mapAnn. rewrite H19.
+      decide (n=n0); subst. repeat get_functional; subst.
+      rewrite H19.
+      revert H20; clear_all; cset_tac; intuition.
+      exploit H3; eauto. eapply zip_get; eauto. eapply zip_get; eauto.
+      unfold defVars in X0. simpl in *.
+      exploit H2; try eapply H12; eauto. dcr. rewrite H22.
+      revert H20 H24; clear_all; cset_tac; intuition; eauto.
+      rewrite List.map_length; eauto.
+      erewrite bounded_restrict_eq; simpl; eauto. simpl.
+      exploit H2; eauto; dcr.
+      rewrite H15. revert H16; clear_all; cset_tac; intuition; eauto.
+    + eapply srd_monotone.
+      eapply (IHrenamedApart (globals F (List.map (mapAnn fst) ans) ++ DL)); eauto.
+      * unfold globals. rewrite app_length, zip_length2; eauto.
+      * pe_rewrite. rewrite List.map_app. rewrite bounded_app. split; eauto.
+        eapply get_bounded.
+        intros. inv_map H9. eapply inv_globals in H10.
+        destruct H10; dcr; subst.
+        inv_map H12. exploit H2; eauto; dcr.
+        rewrite getAnn_mapAnn. rewrite H16.
+        revert H17; clear_all; cset_tac; intuition. rewrite map_length; eauto.
+      * rewrite List.map_app. reflexivity.
 Qed.
 
 (** *** In a coherent program, the globals of every function that can eventually be called are live *)
+
+Lemma eqReq_oglobals_liveGlobals F als
+: length F = length als
+  -> PIR2 eqReq (oglobals F als) (Liveness.live_globals F als).
+Proof.
+  intros. length_equify. general induction H; simpl; eauto using PIR2.
+  - econstructor.
+  - econstructor; eauto.
+    econstructor; reflexivity.
+Qed.
+
+Lemma oglobals_length F als
+: length F = length als
+  -> length (oglobals F als) = length F.
+Proof.
+  intros. unfold oglobals. rewrite map_length.
+  unfold globals. rewrite zip_length2; eauto.
+Qed.
+
+Lemma liveGlobals_length DL
+: length (live_globals DL) = length DL.
+Proof.
+  intros. unfold live_globals. rewrite map_length; eauto.
+Qed.
+
 
 Lemma srd_globals_live s DL AL alv f
 : live_sound Imperative AL s alv
@@ -232,20 +273,28 @@ Proof.
     dcr. edestruct restrict_get; eauto.
     eexists; split; eauto. revert H6; clear_all; cset_tac; intuition; eauto.
     specialize (H6 a); cset_tac; intuition.
-  - edestruct IHsrd1; eauto. econstructor; eauto using restrict_eqReq.
-    destruct if; simpl. econstructor. simpl. reflexivity. econstructor.
-    destruct f; simpl in *. dcr.
-    inv H3.
-    edestruct restrict_get; eauto.
-    edestruct IHsrd2; eauto. econstructor; eauto using restrict_eqReq.
-    econstructor. simpl. reflexivity.
-    simpl in *; dcr. inv H14.
-    eexists; split; eauto. rewrite <- H13, <- H16; eauto.
-  - edestruct IHsrd2; eauto. econstructor; eauto using restrict_eqReq.
-    econstructor. reflexivity.
-    destruct f; simpl in *; dcr.
-    inv H3.
-    eexists; split; eauto. rewrite H4; eauto.
+  - edestruct get_length_eq; eauto.
+    edestruct H1; eauto.
+    rewrite restrict_app. eapply PIR2_app; eauto using restrict_eqReq.
+    eapply restrict_eqReq; eauto using eqReq_oglobals_liveGlobals.
+    dcr. destruct f; simpl in *.
+    edestruct IHsrd; eauto using PIR2_app, restrict_eqReq, eqReq_oglobals_liveGlobals.
+    simpl in *; dcr.
+    rewrite restrict_app in H11.
+    assert (length F = length (restrict (oglobals F als) (getAnn x \ of_list (fst Zs)))).
+    rewrite restrict_length.
+    rewrite oglobals_length; eauto.
+    rewrite H7 in H11. eapply shift_get in H11.
+    eapply restrict_get in H11; dcr.
+    eexists; split; eauto.
+    eapply get_app_le in H19.
+    eapply inv_oglobals in H19. destruct H19; dcr. repeat get_functional; subst.
+    rewrite H22, H20; eauto. eauto. rewrite oglobals_length; eauto.
+  - edestruct IHsrd; eauto using PIR2_app, restrict_eqReq, eqReq_oglobals_liveGlobals.
+    destruct f; simpl in *.
+    dcr.
+    erewrite <- oglobals_length in H7. eapply shift_get in H7.
+    eexists; split; eauto. rewrite H8; eauto. eauto.
 Qed.
 
 (** *** On a coherent program a liveness analysis which is sound imperatively is also sound functionally. *)
@@ -260,22 +309,22 @@ Proof.
   intros. general induction H0; invt live_sound; invt noUnreachableCode; simpl in * |- *;
           eauto using live_sound, restrict_eqReq.
   - econstructor; eauto.
-    + eapply IHsrd1; eauto.
-      econstructor; eauto using restrict_eqReq.
-      destruct if; econstructor; reflexivity.
-    + eapply IHsrd2; eauto.
-      econstructor; eauto using restrict_eqReq.
-      econstructor; reflexivity.
-    + simpl. edestruct srd_globals_live; eauto.
-      econstructor; eauto. econstructor; reflexivity.
-      dcr. inv H3. rewrite H4; eauto.
+    + eapply IHsrd; eauto using PIR2_app, restrict_eqReq, eqReq_oglobals_liveGlobals.
+    + intros. eapply H1; eauto using PIR2_app, restrict_eqReq, eqReq_oglobals_liveGlobals.
+    + intros. exploit H15; eauto; dcr.
+      edestruct srd_globals_live; eauto using PIR2_app, restrict_eqReq, eqReq_oglobals_liveGlobals.
+      eapply H10; eauto. eapply get_length; eauto. dcr.
+      simpl; split; eauto.
+      eapply get_app_le in H18; simpl.
+      eapply inv_oglobals in H18. destruct H18; dcr. simpl in *. repeat get_functional; subst.
+      rewrite H19; eauto. eauto.
+      rewrite oglobals_length; eauto using get_length.
 Qed.
 
 (** ** Definition of invariance *)
 
 Definition invariant (s:stmt) :=
   forall (E:onv var), bisim (nil:list F.block,E,s) (nil:list I.block,E,s).
-
 
 (** ** Agreement Invariant *)
 
@@ -321,144 +370,128 @@ Qed.
 
 (** ** Context coherence for IL/F contexts: [approxF] *)
 
-Inductive approxF
-  : list (option (set var)) -> list (set var * list var) -> F.block -> Prop :=
-  approxI' AL DL o Z E s
+Inductive approx
+  : list (option (set var) * (set var * list var)) -> option (set var) * (set var * list var) -> F.block -> I.block -> Prop :=
+  approxI AL DL o Z E s n lvZ
   :  (forall G, o = Some G -> of_list Z ∩ G [=] ∅ /\
            exists a, getAnn a [=] (G ∪ of_list Z)
-                /\ srd (restrict (Some G::AL) G) s a
+                /\ srd (restrict AL G) s a
                 /\ live_sound Imperative DL s a)
-     -> approxF (o::AL) DL (F.blockI E Z s).
+     -> snd lvZ = Z
+     -> length AL = length DL
+     -> approx (zip pair AL DL) (o, lvZ) (F.blockI E Z s n) (I.blockI Z s n).
 
 (** Stability under restriction *)
 
-Lemma approx_restrict AL DL L G
-: AIR21 approxF AL DL L
-  -> AIR21 approxF (restrict AL G) DL L.
+Lemma zip_eq_app_inv X Y Z (f:X->Y->Z) L L' AL DL
+: length AL = length DL
+  -> L ++ L' = zip f AL DL
+  -> exists AL1 AL2 DL1 DL2,
+      AL = AL1 ++ AL2 /\ DL = DL1 ++ DL2 /\ L = zip f AL1 DL1 /\ L' = zip f AL2 DL2 /\
+      length AL1 = length DL1 /\ length AL2 = length DL2.
 Proof.
-  intros.
-  general induction H; simpl; eauto using AIR21.
-  econstructor. case_eq (restr G x); intros.
-  inv pf. econstructor.
-  intros. inv H1.
-  eapply restr_iff in H0; dcr; subst.
-  specialize (H5 _ H1); dcr.
-  rewrite restrict_incl, restrict_idem, <- restrict_incl; eauto; try reflexivity.
-  inv pf. econstructor. isabsurd. eapply IHAIR21; eauto.
+  intros. general induction L; simpl in *; subst.
+  - eexists nil, AL, nil, DL; simpl; intuition.
+  - destruct AL, DL; simpl in *; isabsurd. inv H0.
+    exploit IHL; try eapply H3. omega. dcr; subst.
+    eexists (x::x0), x1, (y::x2), x3; simpl; intuition.
+Qed.
+
+
+Lemma zip_app X Y Z (f: X -> Y -> Z) L1 L1' L2 L2'
+: length L1 = length L2
+  -> zip f (L1++L1') (L2++L2') = zip f L1 L2 ++ zip f L1' L2'.
+Proof.
+  intros. length_equify.
+  general induction H; simpl; eauto.
+  f_equal; eauto.
 Qed.
 
 Unset Printing Records.
 
-(** ** Preservation properties *)
-(** The rough slogan of what we show here is that the set of coherent states
-    is closed under reduction *)
-
-Lemma srd_preservation (E E':onv val) L L' s s' DL (G:set var) DA a e
-  (SRD:srd DA s a)
-  (RA:rd_agree DA L E)
-  (A: AIR21 approxF DA DL L)
-  (LV:live_sound Imperative DL s a)
-  (S:F.step (L, E, s) e (L',E',s'))
-  : exists DA' DL' a', srd DA' s' a'
-                   /\ rd_agree DA' L' E'
-                   /\ AIR21 approxF DA' DL' L'.
+Lemma zip_eq_cons_inv X Y Z (f:X->Y->Z) a L L1 L2
+:  a :: L = zip f L1 L2
+   -> exists b c L1' L2', b::L1'=L1 /\ c::L2'=L2 /\ a = f b c /\ L = zip f L1' L2'.
 Proof.
-  destruct SRD; try inv S.
-
-  + do 3 eexists; repeat split; try eassumption;
-    eauto using agree_on_update_any_same, approx_restrict, rd_agree_update.
-
-  + do 3 eexists; eauto.
-  + do 3 eexists; eauto.
-
-  + provide_invariants_21. specialize (H3 _ H4); dcr.
-    rewrite H2 in H7. simpl in *.
-    do 3 eexists; repeat split; simpl; eauto.
-    pose proof (RA _ _ _ H1 H). simpl in *.
-    eapply rd_agree_update_list; eauto.
-    exploit omap_length; eauto. rewrite map_length. congruence.
-    eapply approx_restrict; eauto.
-  + do 3 eexists; repeat split; try eassumption;
-    eauto using agree_on_update_any_same, approx_restrict, rd_agree_update.
-
-  + inv LV. do 3 eexists; repeat split; eauto.
-    hnf; intros.
-    destruct n; inv H; inv H0. simpl.
-    reflexivity.
-    eapply RA; eauto.
-
-    econstructor; eauto using agree_on_incl.
-    econstructor; eauto.
-    split. inv H.
-    split; cset_tac; isabsurd; eauto. inv H.
-    eexists; eauto. split; [| split;eauto].
-    cset_tac; intuition. decide (a ∈ of_list Z); intuition.
+  intros. destruct L1, L2; isabsurd.
+  do 4 eexists; intuition; simpl in H; inv H; eauto.
 Qed.
 
-(** context coherence for imperative states (not required in the soundess proof) *)
-
-Inductive approxI
-  : list (option (set var)) -> list (set var * list var) -> I.block -> Prop :=
-  approxII' AL DL o Z s i
-  :  (forall G, o = Some G -> of_list Z ∩ G [=] ∅ /\
-           exists a, getAnn a [=] (G ∪ of_list Z)
-                /\ srd (restrict (Some G::AL) G) s a
-                /\ live_sound i DL s a)
-     -> approxI (o::AL) DL (I.blockI Z s).
-
-Lemma approxI_restrict AL DL L G
-: AIR21 approxI AL DL L
-  -> AIR21 approxI (restrict AL G) DL L.
+Lemma zip_pair_inv X Y (AL1 AL2:list X) (DL1 DL2:list Y)
+: length AL1 = length DL1
+  -> length AL2 = length DL2
+  -> zip pair AL1 DL1 = zip pair AL2 DL2
+  -> AL1 = AL2 /\ DL1 = DL2.
 Proof.
-  intros.
-  general induction H; simpl; eauto using AIR21.
-  econstructor. case_eq (restr G x); intros.
-  inv pf. econstructor.
-  intros. inv H1.
-  eapply restr_iff in H0; dcr; subst.
-  specialize (H5 _ H1); dcr.
-  rewrite restrict_incl, restrict_idem, <- restrict_incl; eauto; try reflexivity.
-  inv pf. econstructor. isabsurd. eapply IHAIR21; eauto.
-  Grab Existential Variables. eapply i.
+  intros. length_equify. general induction H; inv H0; simpl in *; isabsurd; eauto.
+  - inv H1.
+    exploit IHlength_eq; try eapply H5; eauto; dcr; subst; eauto.
 Qed.
 
-Lemma srd_preservation_I (E E':onv val) L L' s s' DL (G:set var) DA a e i
-  (SRD:srd DA s a)
-  (A: AIR21 approxI DA DL L)
-  (LV:live_sound i DL s a)
-  (S:I.step (L, E, s) e (L',E',s'))
-  : exists DL' DA' a', srd DA' s' a' /\ AIR21 approxI DA' DL' L'.
+
+Lemma zip_pair_app_inv X Y (AL AL1 AL2:list X) (DL DL1 DL2:list Y)
+: length AL1 = length DL1
+  -> length AL2 = length DL2
+  -> length AL = length DL
+  -> zip pair AL DL = zip pair (AL1 ++ AL2) (DL1 ++ DL2)
+  -> AL = AL1 ++ AL2 /\ DL = DL1 ++ DL2.
 Proof.
-  destruct SRD; try inv S.
-
-  - do 3 eexists; repeat split; try eassumption;
-    eauto using agree_on_update_any_same, approxI_restrict, rd_agree_update.
-
-  - eexists; eauto.
-  - eexists; eauto.
-
-  - provide_invariants_21.
-    specialize (H3 _ H4); dcr.
-    rewrite H2 in H7. simpl in *.
-    do 3 eexists; repeat split; simpl; eauto using approxI_restrict.
-  - eexists; repeat split; try eassumption;
-    eauto using agree_on_update_any_same, approxI_restrict, rd_agree_update.
-
-  - inv LV. do 3 eexists; repeat split; eauto.
-    econstructor; eauto.
-    econstructor; eauto.
-    split; inv H.
-    + cset_tac; intuition.
-    + eexists; eauto. split; [| split;eauto].
-      * cset_tac; intuition. decide (a ∈ of_list Z); intuition.
+  intros. length_equify. general induction H1.
+  - inv H; inv H0; simpl in *; isabsurd; eauto.
+  - inv H; simpl in *; isabsurd.
+    + inv H0; simpl in *; isabsurd.
+      inv H2. exploit (IHlength_eq nil XL0 nil YL0); eauto. dcr; subst. intuition.
+    + inv H2. exploit (IHlength_eq XL0 AL2 YL0 DL2); eauto. dcr; subst. intuition.
 Qed.
+
+Lemma approx_restrict_block AL1 AL2 DL1 DL2 L1 L2 G n AL1' DL1'
+: length AL1 = length DL1
+  -> length AL2 = length DL2
+  -> mutual_block (approx (zip pair AL1 DL1 ++ zip pair AL2 DL2)) n
+                 (zip pair AL1' DL1') L1 L2
+  -> mutual_block
+      (approx (zip pair (restrict AL1 G) DL1 ++ zip pair (restrict AL2 G) DL2))
+      n (zip pair (restrict AL1' G) DL1') L1 L2.
+Proof.
+  intros. general induction H1.
+  - destruct AL1', DL1'; isabsurd; constructor.
+  - eapply zip_eq_cons_inv in Heql. destruct Heql as [? [? ?]]; eauto; dcr; subst.
+    simpl. econstructor; eauto.
+    inv H2. rewrite <- zip_app; try rewrite restrict_length; eauto.
+    rewrite <- zip_app in H0; eauto.
+    eapply zip_pair_app_inv in H0; dcr; subst; eauto.
+    econstructor; eauto.
+    intros. eapply restr_iff in H0; dcr; subst. exploit H7; eauto; dcr.
+    intuition.
+    eexists x; intuition.
+    rewrite <- restrict_app; eauto. rewrite restrict_idem; eauto.
+    repeat rewrite app_length. repeat rewrite restrict_length. congruence.
+Qed.
+
+Lemma approx_restrict AL DL G L L'
+: length AL = length DL
+  -> inRel approx (zip pair AL DL) L L'
+  -> inRel approx (zip pair (restrict AL G) DL) L L'.
+Proof.
+  intros. length_equify.
+  general induction H0; simpl in *; eauto using inRel.
+  - inv H; isabsurd; econstructor.
+  - eapply zip_eq_app_inv in Heql; eauto using length_eq_length.
+    destruct Heql as [AL1 [AL2 [DL1 [DL2 ?]]]]; dcr; subst.
+    rewrite restrict_app. rewrite zip_app; try rewrite restrict_length; eauto.
+    econstructor. eapply IHinRel; eauto using length_length_eq.
+    eapply approx_restrict_block; eauto.
+Qed.
+
+
+Unset Printing Records.
 
 (** ** Main Theorem about Coherence *)
 
 (** [stripB] removes the environment from a closure  *)
 Definition stripB (b:F.block) : I.block :=
   match b with
-    | F.blockI E Z s => I.blockI Z s
+    | F.blockI E Z s n => I.blockI Z s n
   end.
 
 Definition strip := List.map stripB.
@@ -472,14 +505,65 @@ Qed.
 (** The Bisimulation candidate. *)
 
 Inductive srdSim : F.state -> I.state -> Prop :=
-  | srdSimI (E EI:onv val) L s AL DL a
+  | srdSimI (E EI:onv val) L L' s AL DL a
   (SRD:srd AL s a)
   (RA:rd_agree AL L E)
-  (A: AIR21 approxF AL DL L)
+  (A: inRel approx (zip pair AL DL) L L')
   (AG:agree_on eq (getAnn a) E EI)
   (LV:live_sound Imperative DL s a)
   (ER:PIR2 eqReq AL DL)
-  : srdSim (L, E, s) (strip L, EI,s).
+  : srdSim (L, E, s) (L', EI,s).
+
+
+Lemma zip_zip X X' Y Y' Z (f:X->Y->Z) (g1:X'->Y'->X) (g2:X'->Y'->Y) L L'
+: zip f (zip g1 L L') (zip g2 L L') =
+  zip (fun x y => f (g1 x y) (g2 x y)) L L'.
+Proof.
+  intros. general induction L; destruct L'; simpl; eauto.
+  f_equal; eauto.
+Qed.
+
+Lemma zip_sym X Y Z (f:X->Y->Z) L L'
+: zip f L L' = zip (fun x y => f y x) L' L.
+Proof.
+  general induction L; destruct L'; simpl; eauto.
+  f_equal; eauto.
+Qed.
+
+
+Lemma drop_zip X Y Z (f:X->Y->Z) L L' n
+: length L = length L'
+  -> drop n (zip f L L') = zip f (drop n L) (drop n L').
+Proof.
+  intros. length_equify.
+  general induction H; simpl; eauto.
+  - repeat rewrite drop_nil; eauto.
+  - destruct n; simpl; eauto.
+Qed.
+
+
+Lemma rd_agree_extend F als AL L E
+: length F = length als
+  -> rd_agree AL L E
+  -> rd_agree (oglobals F als ++ AL) (F.mkBlocks E F ++ L) E.
+Proof.
+  intros. hnf; intros.
+  assert (length (F.mkBlocks E F) = length (oglobals F als)).
+  rewrite oglobals_length. unfold F.mkBlocks, mapi. rewrite mapi_length; eauto.
+  eauto.
+  assert (length (oglobals F als) = length F).
+  rewrite oglobals_length; eauto.
+  eapply get_app_cases in H2; eauto. destruct H2.
+  - eapply get_in_range_app in H1; eauto.
+    eapply inv_oglobals in H2; eauto. destruct H2; dcr; subst; eauto.
+    unfold F.mkBlocks in H1. inv_mapi H1. reflexivity.
+    eapply get_length in H2. omega.
+  - dcr.
+    eapply H0; eauto.
+    eapply shift_get; eauto. instantiate (2:=F.mkBlocks E F).
+    orewrite (length (F.mkBlocks E F) + (n - length (oglobals F als)) = n); eauto.
+Qed.
+
 
 (** The bisimulation is indeed a bisimulation *)
 
@@ -492,7 +576,7 @@ Proof.
     one_step.
     instantiate (1:=v). erewrite <- exp_eval_live; eauto.
     eapply srdSim_sim; econstructor;
-    eauto using approx_restrict, rd_agree_update.
+    eauto using approx_restrict, rd_agree_update, PIR2_length.
     eapply agree_on_update_same. reflexivity.
     eapply agree_on_incl; eauto.
     eauto using restrict_eqReq.
@@ -508,65 +592,87 @@ Proof.
     exploit exp_eval_live_agree; eauto.
     no_step.
   - no_step. simpl. eapply exp_eval_live; eauto.
-  - decide (length Z0 = length Y).
+  - decide (length Z = length Y).
     case_eq (omap (exp_eval E) Y); intros.
     + exploit omap_exp_eval_live_agree; eauto.
-      pose proof (map_get_1 stripB H1).
-      one_step.
-      eapply srdSim_sim. rewrite drop_strip.
-      simpl. simpl counted in *.
-      specialize (H4 _ H3); dcr. rewrite H2 in A1,H12.
-      econstructor; simpl; eauto using approx_restrict.
+      exploit (@zip_get _ _ _ pair AL DL); eauto.
+      inRel_invs.
+      one_step. simpl.
+      eapply srdSim_sim.
+      exploit H9; eauto; dcr. simpl in *.
+      econstructor; simpl; eauto using approx_restrict, PIR2_length.
+      assert (restrict AL0 G' = restrict (drop (labN f - n) AL) G').
+      rewrite drop_zip in H2. eapply zip_pair_inv in H2; dcr; subst. reflexivity.
+      eauto. repeat rewrite length_drop_minus. eapply PIR2_length in ER. omega.
+      eauto using PIR2_length.
+      rewrite H11.
       eapply rd_agree_update_list; eauto.
       exploit omap_length; eauto. rewrite map_length. congruence.
       eapply (RA _ _ _ H1 H).
-      eapply update_with_list_agree; eauto. rewrite H11.
+      eapply approx_restrict; eauto.
+      rewrite H2. eapply (inRel_drop A H1).
+      eapply update_with_list_agree; eauto. rewrite H8.
       rewrite union_comm. rewrite union_minus_remove.
       pose proof (RA _ _ G' H1 H); dcr. simpl in *.
       eapply agree_on_sym; eauto. eapply agree_on_incl; eauto using incl_minus.
       etransitivity; eauto. symmetry. hnf in RA.
       eapply agree_on_incl; eauto.
       edestruct PIR2_nth_2; eauto; dcr. get_functional; eauto; subst.
-      inv H16. rewrite H13. simpl. eauto.
+      inv H16. rewrite H14. simpl. eauto.
       exploit omap_length; eauto. rewrite map_length. congruence.
-      eapply restrict_eqReq. eapply PIR2_drop; eauto.
+      eapply restrict_eqReq.
+      rewrite drop_zip in H2; eauto using PIR2_length.
+      eapply  zip_pair_inv in H2; dcr; subst; eauto.
+      eapply PIR2_drop; eauto.
+      repeat rewrite length_drop_minus. eapply PIR2_length in ER; eauto.
     + exploit omap_exp_eval_live_agree; eauto.
       no_step.
-    + no_step. get_functional; subst; simpl in *; congruence.
-      unfold strip in *.
-      edestruct map_get_4; eauto; dcr; get_functional; subst; simpl in *.
-      congruence.
+    + no_step.
   - case_eq (omap (exp_eval E) Y); intros;
     exploit omap_exp_eval_live_agree; eauto.
     extern_step; assert (vl = l) by congruence; subst.
     + eexists; split. econstructor; eauto.
-      eapply srdSim_sim; econstructor; eauto using approx_restrict, rd_agree_update.
+      eapply srdSim_sim; econstructor; eauto using approx_restrict, rd_agree_update, PIR2_length.
       eapply agree_on_update_same. reflexivity.
       eapply agree_on_incl; eauto.
       eauto using restrict_eqReq; eauto.
     + symmetry in AG.
       exploit omap_exp_eval_live_agree; eauto.
       eexists; split. econstructor; eauto.
-      eapply srdSim_sim; econstructor; eauto using approx_restrict, rd_agree_update.
+      eapply srdSim_sim; econstructor; eauto using approx_restrict, rd_agree_update, PIR2_length.
       eapply agree_on_update_same. reflexivity.
       symmetry in AG.
       eapply agree_on_incl; eauto.
       eauto using restrict_eqReq; eauto.
     + no_step.
   - one_step.
-    eapply srdSim_sim; econstructor; eauto.
-    hnf; intros.
-    destruct n; inv H1; inv H2. simpl.
-    reflexivity.
-    eapply RA; eauto.
-
-    econstructor; eauto using agree_on_incl. econstructor; eauto.
-    intros. inv H1. split.
-    split; cset_tac; isabsurd; eauto.
-    eexists. split; eauto. cset_tac; intuition.
-    decide (a ∈ of_list Z); intuition.
-    eapply agree_on_incl; eauto.
-    econstructor; eauto. econstructor; reflexivity.
+    eapply srdSim_sim; econstructor;
+    eauto using agree_on_incl, PIR2_app, eqReq_oglobals_liveGlobals, rd_agree_extend.
+    rewrite zip_app. econstructor; eauto.
+    unfold F.mkBlocks, I.mkBlocks. unfold mapi.
+    unfold oglobals at 2. unfold globals.
+    unfold Liveness.live_globals at 2.
+    unfold Liveness.live_global.
+    rewrite map_zip. rewrite zip_zip.
+    erewrite (zip_sym _ F als).
+    eapply mutual_approx; simpl; eauto; try congruence.
+    intros. simpl. rewrite <- zip_app. econstructor; eauto.
+    intros. inv H4. simpl. unfold global. simpl.
+    split. clear_all; cset_tac; intuition.
+    eexists a. split.
+    exploit H11; eauto. dcr; simpl in *.
+    revert H5; clear_all; cset_tac; intuition.
+    decide (a0 ∈ of_list Z); intuition.
+    split. exploit H0; eauto.
+    exploit H10; eauto.
+    repeat rewrite app_length.
+    unfold Liveness.live_globals; rewrite zip_length2.
+    rewrite oglobals_length; eauto. eapply PIR2_length in ER. omega.
+    eauto.
+    unfold Liveness.live_globals; rewrite zip_length2.
+    rewrite oglobals_length; eauto. eauto.
+    unfold Liveness.live_globals; rewrite zip_length2.
+    rewrite oglobals_length; eauto. eauto.
 Qed.
 
 (** ** Coherence implies invariance *)
@@ -575,9 +681,8 @@ Lemma srd_implies_invariance s a
 : live_sound Imperative nil s a -> srd nil s a -> invariant s.
 Proof.
   intros. hnf; intros. eapply srdSim_sim.
-  econstructor; eauto using AIR21, PIR2; isabsurd.
+  econstructor; eauto. isabsurd. econstructor. econstructor.
 Qed.
-
 
 (*
 *** Local Variables: ***
